---
course: ''
course_year: IA
question_number: 29
tags:
- IA
- '2016'
- ''
title: Paper 4, Section II
year: 2016
---


8E Numbers and Sets

Define the binomial coefficient $\left(\begin{array}{c}n \\ m\end{array}\right)$. Prove directly from your definition that

$$(1+z)^{n}=\sum_{m=0}^{n}\left(\begin{array}{c}
n \\
m
\end{array}\right) z^{m}$$

for any complex number $z$.

(a) Using this formula, or otherwise, show that

$$\sum_{k=0}^{3 n}(-3)^{k}\left(\begin{array}{l}
6 n \\
2 k
\end{array}\right)=2^{6 n}$$

(b) By differentiating, or otherwise, evaluate $\sum_{m=0}^{n} m\left(\begin{array}{c}n \\ m\end{array}\right)$.

Let $S_{r}(n)=\sum_{m=0}^{n}(-1)^{m} m^{r}\left(\begin{array}{c}n \\ m\end{array}\right)$, where $r$ is a non-negative integer. Show that $S_{r}(n)=0$ for $r<n$. Evaluate $S_{n}(n)$.