---
course: Integrable Systems
course_year: II
question_number: 79
tags:
- II
- '2020'
- Integrable Systems
title: 'Paper 1, Section II, 33C '
year: 2020
---



(a) Show that if $L$ is a symmetric matrix $\left(L=L^{T}\right)$ and $B$ is skew-symmetric $\left(B=-B^{T}\right)$ then $[B, L]=B L-L B$ is symmetric.

(b) Consider the real $n \times n$ symmetric matrix

$$L=\left(\begin{array}{cccccccc}
0 & a_{1} & 0 & 0 & \cdots & \cdots & \cdots & 0 \\
a_{1} & 0 & a_{2} & 0 & \cdots & \cdots & \cdots & 0 \\
0 & a_{2} & 0 & a_{3} & \cdots & \cdots & \cdots & 0 \\
0 & 0 & a_{3} & \cdots & \cdots & \cdots & \cdots & 0 \\
\cdots & \cdots & \cdots & \cdots & \cdots & \cdots & \cdots & \cdots \\
0 & \cdots & \cdots & \cdots & \cdots & \cdots & a_{n-2} & 0 \\
0 & \cdots & \cdots & \cdots & \cdots & a_{n-2} & 0 & a_{n-1} \\
0 & \cdots & \cdots & \cdots & \cdots & 0 & a_{n-1} & 0
\end{array}\right)$$

(i.e. $L_{i, i+1}=L_{i+1, i}=a_{i}$ for $1 \leqslant i \leqslant n-1$, all other entries being zero) and the real $n \times n$ skew-symmetric matrix

$$B=\left(\begin{array}{cccccccc}
0 & 0 & a_{1} a_{2} & 0 & \cdots & \cdots & \cdots & 0 \\
0 & 0 & 0 & a_{2} a_{3} & \cdots & \ldots & \ldots & 0 \\
-a_{1} a_{2} & 0 & 0 & 0 & \ldots & \ldots & \ldots & 0 \\
0 & -a_{2} a_{3} & 0 & \ldots & \cdots & \ldots & \ldots & 0 \\
\ldots & \ldots & \ldots & \ldots & \ldots & \ldots & \ldots & \ldots \\
0 & \ldots & \ldots & \ldots & \ldots & \ldots & 0 & a_{n-2} a_{n-1} \\
0 & \ldots & \cdots & \cdots & \cdots & 0 & 0 & 0 \\
0 & \ldots & \cdots & \cdots & \ldots & -a_{n-2} a_{n-1} & 0 & 0
\end{array}\right)$$

(i.e. $B_{i, i+2}=-B_{i+2, i}=a_{i} a_{i+1}$ for $1 \leqslant i \leqslant n-2$, all other entries being zero).

(i) Compute $[B, L]$.

(ii) Assume that the $a_{j}$ are smooth functions of time $t$ so the matrix $L=L(t)$ also depends smoothly on $t$. Show that the equation $\frac{d L}{d t}=[B, L]$ implies that

$$\frac{d a_{j}}{d t}=f\left(a_{j-1}, a_{j}, a_{j+1}\right)$$

for some function $f$ which you should find explicitly.

(iii) Using the transformation $a_{j}=\frac{1}{2} \exp \left[\frac{1}{2} u_{j}\right]$ show that

$$\frac{d u_{j}}{d t}=\frac{1}{2}\left(e^{u_{j+1}}-e^{u_{j-1}}\right)$$

for $j=1, \ldots n-1$. [Use the convention $u_{0}=-\infty, a_{0}=0, u_{n}=-\infty, a_{n}=0 .$ ]

(iv) Deduce that given a solution of equation ( $\dagger$, there exist matrices $\{U(t)\}_{t \in \mathbb{R}}$ depending on time such that $L(t)=U(t) L(0) U(t)^{-1}$, and explain how to obtain first integrals for $(t)$ from this.